feat : ex3 termination of type check & evaluation

mini-spec/ex3-global-and-decl/ex3spec.v
@@ -19,6 +19,50 @@ Inductive type :=
     | INT
     | Func (ty1 ty2 : type)
     | REF (ty : type).
+    
+Fixpoint type_eq (ty1 ty2 : type) : bool := match ty1, ty2 with
+| INT, INT => true
+| Func ty11 ty12, Func ty21 ty22 => andb (type_eq ty11 ty21) (type_eq ty12 ty22)
+| REF ty1, REF ty2 => type_eq ty1 ty2
+| _, _ => false
+end.
+
+Theorem Type_Eq_is_valid1 : forall ty1 ty2, type_eq ty1 ty2 = true <-> ty1 = ty2.
+Proof.
+    intro ty1. induction ty1; intro ty2.
+    {
+        split.
+        + destruct ty2; intro E; try (simpl in E; discriminate E); reflexivity.
+        + destruct ty2;  intro E; try (simpl in E; discriminate E); reflexivity.
+    }
+    {
+        split.
+        + destruct ty2; intro E; try (simpl in E; discriminate E).
+          - simpl in E.
+            destruct (type_eq ty1_1 ty2_1) eqn:E1; try (discriminate E).
+            destruct (type_eq ty1_2 ty2_2) eqn:E2; try (discriminate E).
+            rewrite IHty1_1 in E1. rewrite IHty1_2 in E2.
+            f_equal. apply E1. apply E2.
+        + destruct ty2; intro E; try (simpl in E; discriminate E).
+          - injection E as E1 E2. rewrite <- IHty1_1 in E1. rewrite <- IHty1_2 in E2.
+            simpl. rewrite E1, E2. reflexivity.
+    }
+    {
+        split.
+        + destruct ty2; intro E; try (simpl in E; discriminate E).
+          - simpl in E. rewrite IHty1 in E. f_equal. apply E.
+        + destruct ty2; intro E; try (simpl in E; discriminate E).
+          - injection E as E. rewrite <- IHty1 in E. simpl. apply E.
+    }
+Qed.
+
+Theorem Type_Eq_is_valid2 : forall ty, type_eq ty ty = true.
+Proof.
+    intro ty.
+    induction ty; try reflexivity.
+    - simpl. rewrite IHty1, IHty2. reflexivity.
+    - simpl. rewrite IHty. reflexivity.
+Qed.
 
 Inductive expr :=
     | NumE (n : nat)
@@ -48,9 +92,9 @@ Inductive Typing : context -> expr -> type -> Prop :=
         (C |- el : INT) -> (C |- er : INT) -> C |- (BinE op el er) : INT
     | T_letE : forall CG CL x ep eb typ tyb,
         ((CG, CL) |- ep : typ) -> ((CG, ((x, typ) :: CL)) |- eb : tyb) -> (CG, CL) |- (LetE x ep eb) : tyb
-    | T_varE_local : forall CG CL x ty, 
-        (find_id x CG = Some ty) -> (CG, CL) |- (VarE x) : ty
     | T_varE_global : forall CG CL x ty, 
+        (find_id x CG = Some ty) -> (CG, CL) |- (VarE x) : ty
+    | T_varE_local : forall CG CL x ty, 
         (find_id x CL = Some ty) -> (CG, CL) |- (VarE x) : ty
     | T_funcE : forall CG CL x typ eb tyb,
         ((CG, ((x, typ) :: CL)) |- eb : tyb) -> (CG, CL) |- (FuncE x typ eb) : (Func typ tyb)
@@ -62,6 +106,109 @@ Inductive Typing : context -> expr -> type -> Prop :=
         (C |- el : (REF ty)) -> (C |- er : ty) -> (C |- UpdateE el er : ty)
 where "C |- e : t" := (Typing C e t).
 
+Fixpoint type_check (C : context) (exp : expr) : option type :=
+    match exp with
+    | NumE n => Some INT
+    | BinE _ exp1 exp2 =>
+        match (type_check C exp1), (type_check C exp2) with
+        | Some INT, Some INT => Some INT
+        | _, _ => None
+        end
+    | LetE x exp1 exp2 =>
+        let (CG, CL) := C in
+        match type_check (CG, CL) exp1 with
+        | Some typ => type_check (CG, (x, typ) :: CL) exp2
+        | None => None
+        end
+    | VarE x =>
+        (*erroneous case*)
+        let (CG, CL) := C in
+        match find_id x CG with
+        | Some ty => Some ty
+        | None => find_id x CL
+        end
+    | FuncE x typ exp =>
+        let (CG, CL) := C in
+        match type_check (CG, (x, typ) :: CL) exp with
+        | Some tyb => Some (Func typ tyb)
+        | None => None
+        end
+    | ApplyE exp1 exp2 =>
+        match type_check C exp1 with
+        | Some (Func typ tyb) => 
+            match type_check C exp2 with
+            | Some ty => if type_eq typ ty then Some tyb else None
+            | None => None
+            end
+        | _ => None
+        end
+    | RefE exp =>
+        match type_check C exp with
+        | Some ty => Some (REF ty)
+        | None => None
+        end
+    | DerefE exp =>
+        match type_check C exp with
+        | Some (REF ty) => Some ty
+        | _ => None
+        end
+    | UpdateE exp1 exp2 =>
+        match type_check C exp1 with
+        | Some (REF ty1) =>
+            match type_check C exp2 with
+            | Some ty2 => if type_eq ty1 ty2 then Some ty1 else None
+            | None => None
+            end
+        | _ => None
+        end
+    end.
+
+Theorem Termination_Type_Check :
+forall C exp typ, type_check C exp = Some typ -> (C |- exp : typ).
+Proof.
+    intros C exp. generalize dependent C.
+    induction exp; intros C typ E; simpl in E.
+    - injection E as E. rewrite <- E. apply T_numE.
+    - destruct (type_check C exp1) eqn:E1; try (discriminate E).
+      destruct t; try (discriminate E).
+      destruct (type_check C exp2) eqn:E2; try (discriminate E).
+      destruct t; try (discriminate E).
+      apply IHexp1 in E1. apply IHexp2 in E2. injection E as E. rewrite <- E.
+      apply T_binE; assumption.
+    - destruct C as [CG CL].
+      destruct (type_check (CG, CL) exp1) eqn:E1; try (discriminate E).
+      apply IHexp1 in E1. apply IHexp2 in E.
+      apply T_letE with t; assumption.
+    - destruct C as [CG CL].
+      destruct (find_id x CG) eqn:EG.
+      + injection E as E. rewrite <- E. apply T_varE_global; assumption.
+      + apply T_varE_local; assumption.
+    - destruct C as [CG CL].
+      destruct (type_check (CG, (x, ty) :: CL) exp) eqn:Ef; try (discriminate E).
+      injection E as E. rewrite <- E. apply IHexp in Ef. 
+      apply T_funcE; assumption.
+    - destruct (type_check C exp1) eqn:E1; try (discriminate E).
+      destruct t; try (discriminate E).
+      destruct (type_check C exp2) eqn:E2; try (discriminate E).
+      destruct (type_eq t1 t) eqn:Eb; try (discriminate E).
+      rewrite Type_Eq_is_valid1 in Eb. rewrite <- Eb in E2. apply IHexp1 in E1. apply IHexp2 in E2.
+      injection E as E. rewrite <- E. apply T_applyE with t1; assumption.
+    - destruct (type_check C exp) eqn:E1; try (discriminate E).
+      injection E as E. rewrite <- E. apply IHexp in E1.
+      apply T_refE; assumption.
+    - destruct (type_check C exp) eqn:E1; try (discriminate E).
+      destruct t; try (discriminate E).
+      injection E as E. rewrite <- E. apply IHexp in E1.
+      apply T_derefE; assumption.
+    - destruct (type_check C exp1) eqn:E1; try (discriminate E).
+      destruct t; try (discriminate E).
+      destruct (type_check C exp2) eqn:E2; try (discriminate E).
+      destruct (type_eq t t0) eqn:Eb; try (discriminate E).
+      rewrite Type_Eq_is_valid1 in Eb. injection E as E. apply IHexp1 in E1. apply IHexp2 in E2.
+      rewrite <- E. rewrite <- Eb in E2.
+      apply T_updateE; assumption.
+Qed.
+
 Reserved Notation "C |- p ; t" (at level 80, p at next level, t at next level).
 
 Inductive Typing_Prog : context -> program -> type -> Prop :=
@@ -69,6 +216,33 @@ Inductive Typing_Prog : context -> program -> type -> Prop :=
     | T_P_decl : forall CG CL x e p ty typ,
         ((CG, CL) |- e : ty) -> ((((x, ty) :: CG), CL) |- p ; typ) -> (CG, CL) |- (GlobalDecl (GlobalID x e) p) ; typ
 where "C |- p ; t" := (Typing_Prog C p t).
+
+Fixpoint type_check_prog (C : context) (p : program) : option type :=
+    match p with
+    | GlobalDecl gd p' =>
+        let (CG, CL) := C in
+        match gd with
+        | GlobalID x exp =>
+            match type_check C exp with
+            | Some ty =>
+                type_check_prog ((x, ty) :: CG, CL) p'
+            | None => None
+            end
+        end
+    | LocalDecl exp => type_check C exp
+    end.
+
+Theorem Termination_Type_Check_Program :
+forall C p ty, type_check_prog C p = Some ty -> C |- p ; ty.
+Proof.
+    intros C p. generalize dependent C.
+    induction p; intros C ty E; simpl in E.
+    - destruct C as [CG CL]. destruct gd as [x exp].
+      destruct (type_check (CG, CL) exp) eqn:E1; try (discriminate E).
+      apply IHp in E. apply Termination_Type_Check in E1.
+      apply T_P_decl with t; assumption.
+    - apply Termination_Type_Check in E. apply T_P_expr; assumption.
+Qed.
 
 Inductive value :=
     | NumV (n : nat)
@@ -112,17 +286,173 @@ Inductive Eval : environment -> sto -> expr -> value -> sto -> Prop :=
   | E_applyE : forall env env_cloG env_cloL sto sto1 sto2 sto3 x ef ea eb valr vala,
     (env ; sto |- ef ==> (CloV x eb (env_cloG, env_cloL)) ; sto1) -> (env ; sto1 |- ea ==> vala ; sto2) -> ((env_cloG, ((x, vala) :: env_cloL)) ; sto2 |- eb ==> valr ; sto3) -> env ; sto |- (ApplyE ef ea) ==> valr ; sto3
   | E_refE : forall env sto sto1 exp n value,
-    (env ; sto |- exp ==> value ; sto1) -> (length sto = n) -> env ; sto |- (RefE exp) ==> (LocV n) ; (sto1 ++ [ value ])
+    (env ; sto |- exp ==> value ; sto1) -> (length sto1 = n) -> env ; sto |- (RefE exp) ==> (LocV n) ; (sto1 ++ [ value ])
   | E_derefE : forall env sto sto1 exp n value,
     (env ; sto |- exp ==> LocV n ; sto1) -> (find_nth n sto1 = Some value) -> env ; sto |- (DerefE exp) ==> value ; sto1
   | E_updateE : forall env sto sto1 sto2 sto3 el er n valr,
     (env ; sto |- el ==> (LocV n); sto1) -> (env ; sto1 |- er ==> valr ; sto2) -> (change_nth n valr sto2 = sto3) -> env ; sto |- (UpdateE el er) ==> valr ; sto3
 where "C ; St |- e ==> v ; St'" := (Eval C St e v St').
 
+Fixpoint evaluation_w_fuel (env : environment) (st : sto) (exp : expr) (fuel : nat) : option (value * sto) :=
+    match fuel with
+    | 0 => None
+    | S fuel' =>
+        match exp with
+        | NumE n => Some (NumV n, st)
+        | BinE op exp1 exp2 =>
+            match (evaluation_w_fuel env st exp1 fuel') with
+            | Some (NumV n1, st1) =>
+                match (evaluation_w_fuel env st1 exp2 fuel') with
+                | Some (NumV n2, st2) =>
+                    match op with
+                    | ADD => Some (NumV (n1 + n2), st2)
+                    | MUL => Some (NumV (n1 * n2), st2)
+                    end
+                | _ => None
+                end
+            | _ => None
+            end
+        | LetE x exp1 exp2 =>
+            let (envG, envL) := env in
+            match (evaluation_w_fuel (envG, envL) st exp1 fuel') with
+            | Some (valp, st1) => evaluation_w_fuel (envG, (x, valp) :: envL) st1 exp2 fuel'
+            | None => None
+            end
+        | VarE x =>
+            let (envG, envL) := env in
+            match (find_id x envG) with
+            | Some value => Some (value, st)
+            | None => 
+                match (find_id x envL) with
+                | Some value => Some (value, st)
+                | None => None
+                end
+            end
+        | FuncE x ty exp => Some (CloV x exp env, st)
+        | ApplyE exp1 exp2 =>
+            match (evaluation_w_fuel env st exp1 fuel') with
+            | Some (CloV x exp env_clo, st1) =>
+                let (env_cloG, env_cloL) := env_clo in
+                match (evaluation_w_fuel env st1 exp2 fuel') with
+                | Some (vala, st2) =>
+                    evaluation_w_fuel (env_cloG, (x, vala) :: env_cloL) st2 exp fuel'
+                | None => None
+                end
+            | _ => None
+            end
+        | RefE exp =>
+            match evaluation_w_fuel env st exp fuel' with
+            | Some (value, st1) => Some (LocV (length st1), st1 ++ [value])
+            | None => None
+            end
+        | DerefE exp =>
+            match evaluation_w_fuel env st exp fuel' with
+            | Some (LocV n, st1) => 
+                match find_nth n st1 with
+                | Some value => Some (value, st1)
+                | None => None
+                end
+            | _ => None
+            end
+        | UpdateE exp1 exp2 =>
+            match evaluation_w_fuel env st exp1 fuel' with
+            | Some (LocV n, st1) =>
+                match evaluation_w_fuel env st1 exp2 fuel' with
+                | Some (valr, st2) =>
+                    Some (valr, change_nth n valr st2)
+                | None => None
+                end
+            | _ => None
+            end
+        end
+    end.
+
+Theorem Termination_Evaluation :
+forall fuel exp env st1 st2 val, evaluation_w_fuel env st1 exp fuel = Some (val, st2) -> env ; st1 |- exp ==> val ; st2.
+Proof.
+    intro fuel.
+    induction fuel.
+    - intros exp env st1 st2 val E. simpl in E. discriminate E.
+    - intro exp. induction exp; intros env st1 st2 val E; simpl in E.
+      + injection E as Evalue Estate. rewrite <- Evalue, <- Estate. apply E_numE.
+      + destruct (evaluation_w_fuel env st1 exp1 fuel) eqn:E1; try (discriminate E).
+        destruct p as [v sta]. destruct v; try (discriminate E).
+        destruct (evaluation_w_fuel env sta exp2 fuel) eqn:E2; try (discriminate E).
+        destruct p as [v stb]. destruct v; try (discriminate E).
+        apply IHfuel in E1, E2.
+        destruct op.
+        injection E as Evalue Estate. rewrite <- Evalue, <- Estate.
+        apply E_binE_add with sta; assumption.
+        injection E as Evalue Estate. rewrite <- Evalue, <- Estate.
+        apply E_binE_mul with sta; assumption.
+      + destruct env as [envG envL].
+        destruct (evaluation_w_fuel (envG, envL) st1 exp1 fuel) eqn:E1; try (discriminate E).
+        destruct p as [valp sta].
+        apply IHfuel in E, E1. apply E_letE with sta valp; assumption.
+      + destruct env as [envG envL].
+        destruct (find_id x envG) eqn:EG.
+        injection E as Evalue Estate. rewrite <- Evalue, <- Estate. apply E_varE_global; assumption.
+        destruct (find_id x envL) eqn:EL; try (discriminate E).
+        injection E as Evalue Estate. rewrite <- Evalue, <- Estate. apply E_varE_local; assumption.
+      + injection E as Evalue Estate. rewrite <- Evalue, <- Estate. apply E_funcE; assumption.
+      + destruct (evaluation_w_fuel env st1 exp1 fuel) eqn:E1; try (discriminate E).
+        destruct p as [v sta]. destruct v; try (discriminate E). destruct env0 as [env_cloG env_cloL]. 
+        destruct (evaluation_w_fuel env sta exp2 fuel) eqn:E2; try (discriminate E).
+        destruct p as [vala stb].
+        apply IHfuel in E1, E2, E. 
+        apply E_applyE with env_cloG env_cloL sta stb x exp vala; assumption.
+      + destruct (evaluation_w_fuel env st1 exp fuel) eqn:E1; try (discriminate E).
+        destruct p as [value0 sta]. injection E as Evalue Estate. apply IHfuel in E1.
+        rewrite <- Evalue, <- Estate. assert (H : (Datatypes.length sta) = (Datatypes.length sta)). { reflexivity. }
+        apply E_refE; assumption.
+      + destruct (evaluation_w_fuel env st1 exp fuel) eqn:E1; try (discriminate E).
+        destruct p as [v sta]. destruct v; try (discriminate E).
+        destruct (find_nth loc sta) eqn:Efind; try (discriminate E).
+        injection E as Evalue Estate. rewrite <- Evalue, <- Estate. apply IHfuel in E1.
+        apply E_derefE with loc; assumption.
+      + destruct (evaluation_w_fuel env st1 exp1 fuel) eqn:E1; try (discriminate E).
+        destruct p as [v sta]. destruct v; try (discriminate E).
+        destruct (evaluation_w_fuel env sta exp2 fuel) eqn:E2; try (discriminate E).
+        destruct p as [valr stb]. injection E as Evalue Estate. rewrite <- Evalue.
+        apply IHfuel in E1, E2.
+        apply E_updateE with sta stb loc; assumption.
+Qed.
+
 Reserved Notation "C ; St |- p :==> v ; St'"  (at level 80, St at next level, p at next level, v at next level).
 Inductive Eval_Prog : environment -> sto -> program -> value -> sto -> Prop :=
+    | E_expr : forall env st1 st2 e value,
+        (env ; st1 |- e ==> value ; st2) -> env ; st1 |- (LocalDecl e) :==> value ; st2
     | E_decl : forall st st1 st2 envG envL x e p val valp,
         ((envG, envL) ; st |- e ==> val ; st1) ->
         (((x, val) :: envG, envL) ; st1 |- p :==> valp ; st2) ->
         (envG, envL) ; st |- (GlobalDecl (GlobalID x e) p) :==> valp ; st2
 where "C ; St |- p :==> v ; St'" := (Eval_Prog C St p v St').
+
+Fixpoint evaluation_w_fuel_program (env : environment) (st : sto) (p : program) (fuel : nat) {struct fuel} : option (value * sto) :=
+    match fuel with
+    | 0 => None
+    | S fuel' =>
+        match p with
+        | LocalDecl exp => evaluation_w_fuel env st exp fuel'
+        | GlobalDecl (GlobalID x exp) p' =>
+            let (envG, envL) := env in
+            match evaluation_w_fuel (envG, envL) st exp fuel' with
+            | Some (val, st1) => (evaluation_w_fuel_program ((x, val) :: envG, envL) st1 p' fuel')
+            | None => None
+            end
+        end
+    end.
+
+Theorem Termination_Evaluation_Program :
+forall fuel p env st1 st2 value, evaluation_w_fuel_program env st1 p fuel = Some (value, st2) -> env ; st1 |- p :==> value ; st2.
+Proof.
+    intro fuel.
+    induction fuel.
+    - intros p env st1 st2 value E. discriminate E.
+    - intro p. induction p; intros env st1 st2 value E; simpl in E.
+      + destruct gd. destruct env as [envG envL].
+        destruct (evaluation_w_fuel (envG, envL) st1 exp fuel) eqn:E1; try (discriminate E).
+        destruct p0 as [val sta]. apply IHfuel in E. apply Termination_Evaluation in E1.
+        apply E_decl with sta val; assumption.
+      + apply Termination_Evaluation in E. apply E_expr; assumption.
+Qed.
